rocq-osiris/theories/program_logic/rules/basic_rules.v
@@ -1,5 +1,6 @@
 From Stdlib Require Import Program.Equality.
 From iris.base_logic.lib Require Import fancy_updates gen_heap.
+From iris.bi Require Import derived_laws.
 From iris.proofmode Require Import proofmode.
 
 From iris.base_logic.lib Require Import own.
@@ -19,6 +20,188 @@ From osiris.program_logic.pure Require Export pure.
   (1) How to reason about expressions at the [micro] monad level and
   (2) Proof that the weakest precondition is closed under [simp]
       (see [ewp_simp]). *)
+
+(* ------------------------------------------------------------------------ *)
+Section ewp.
+  Import ewp_rules_tactics.
+
+  Context `{!osirisGS Σ}.
+  Context {A X : Type}.
+  Implicit Type m : micro A X.
+
+  (* ------------------------------------------------------------------------ *)
+
+  Lemma ewp_step {E Ψ Q} {σ π σ'} m m' μ :
+    thread_step (σ, m, dom π) (σ', m', μ) →
+    state_interp (σ, π) -∗
+    ewp_def E m Ψ Q ==∗
+    |={E}[∅]▷=>
+        ewp_def E m' Ψ Q ∗
+          (match μ with
+           | None => state_interp (σ', π)
+           | Some (ι', m') => ∃ φ' γ, state_interp (σ', <[ι':= γ]>π) ∗
+                                        saved_prop.saved_pred_own γ DfracDiscarded φ' ∗
+                                        ewp_def ⊤ m' ⊥ (λ o, □ φ' o)
+          end).
+  Proof.
+    intros Hstep.
+    iIntros "Hsi Hwp".
+    ewp_unfold m.
+    ewp_case m.
+    spec_state. iModIntro. iMod "Hwp" as "[%Hprog Hwp]".
+    spec_step.
+    by ewp_mask_elim.
+  Qed.
+
+  (* ------------------------------------------------------------------------ *)
+
+  (** Monotonicity. *)
+  Lemma ewp_strong_mono E1 E2 m Ψ1 Ψ2 Q' Q :
+    E1 ⊆ E2 →
+    ewp_def E1 m Ψ1 Q' -∗
+    (Ψ1 ⊑ Ψ2)%ieff -∗
+    (∀ o, Q' o ={E2}=∗ Q o) -∗
+    ewp_def E2 m Ψ2 Q.
+  Proof.
+    iIntros (HE) "Hwp #Hmonoprot Hmono".
+    iLöb as "IH" forall (m).
+    ewp_unfold m.
+    ewp_case m.
+    (* Case: [m] is a [WPOutcome] *)
+    { iApply ("Hmono" with "[> -]").
+      by iApply (fupd_mask_mono E1 _). }
+
+    (* Case: [m] is a [WPCrash]. *)
+    { by iApply (fupd_mask_mono E1 _). }
+
+    { (* Case: [m] is a [WPPerform]. We use [prot_mono]. *)
+      iApply (fupd_mask_mono E1 _). set_solver.
+      iMod "Hwp"; iModIntro.
+      iDestruct "Hwp" as (φ) "(Hwp & HΨ)"; iExists φ.
+      iSplitL "Hwp"; first iApply ("Hmonoprot" with "Hwp"); cbn.
+      iIntros (?) "Hφ". iSpecialize ("HΨ" with "Hφ").
+      iNext; iApply ("IH" with "HΨ Hmono"). }
+
+    { (* Case: [m] is a [WPStep]. *)
+      intro_state. iMod (fupd_mask_subseteq E1) as "Hmod". set_solver.
+      spec_state. iModIntro.
+      discharge_pure assumption.
+      clear Hstep.
+      iIntros (σ' m' μ) "%Hstep".
+      spec_step.
+      ewp_mask_elim. iMod "Hwp" as "(Hwp & Hforked)". iFrame.
+      iMod "Hmod".
+      iApply ("IH" with "Hwp Hmono"). }
+
+    { (* Case: [m] is a [WPJoin]. *)
+      intro_state. iMod (fupd_mask_subseteq E1) as "Hmod". set_solver.
+      spec_state.
+      iMod "Hwp". iModIntro.
+      destruct (π !! t) eqn:Hlookup.
+      - iDestruct "Hwp" as "(%φ'0 & $ & Hwp)".
+        iIntros "!> %o Ho". iSpecialize ("Hwp" with "Ho").
+        ewp_mask_elim. iMod "Hwp" as "(Hwp & Hforked)". iFrame.
+        iMod "Hmod".
+        iApply ("IH" with "Hwp Hmono").
+      - iMod "Hwp". by iMod "Hmod". }
+  Qed.
+
+  Local Tactic Notation "ewp_mono" "with" constr(s) :=
+    iApply (ewp_strong_mono with s); auto; first iApply iEff_le_refl.
+
+  Lemma ewp_prot_mono E m Ψ1 Ψ2 Q :
+    (Ψ1 ⊑ Ψ2)%ieff -∗
+    ewp_def E m Ψ1 Q -∗
+    ewp_def E m Ψ2 Q.
+  Proof. iIntros "Hprot Hm". iApply (ewp_strong_mono E E with "Hm Hprot"); auto. Qed.
+
+  Lemma fupd_ewp E m Ψ Q :
+    (|={E}=> ewp_def E m Ψ Q) ⊢ ewp_def E m Ψ Q.
+  Proof.
+    iIntros "He".
+    ewp_unfold_all.
+    ewp_case m; try iMod "He"; done.
+  Qed.
+
+  (* Eliminate update modality in postcondition *)
+  Lemma ewp_fupd E m Ψ Q :
+    ewp_def E m Ψ (λ o, |={E}=> Q o) -∗
+    ewp_def E m Ψ Q.
+  Proof. iIntros "He". ewp_mono with "He". Qed.
+
+  Lemma ewp_atomic E E2 m Ψ Q `{!thread_step.Atomic m} :
+    (* TCEq (to_eff m) None → *)
+    (* TCEq (to_join m) None → *)
+    (|={E,E2}=> ewp_def E2 m Ψ (λ o, |={E2,E}=> Q o)) ⊢ ewp_def E m Ψ Q.
+  Proof.
+    iIntros "Hm".
+    ewp_unfold_all.
+    ewp_case m.
+    { by iDestruct "Hm" as ">>> $". }
+    { by iDestruct "Hm" as ">> []". }
+    { admit. }
+    { intro_state.
+      iMod "Hm".
+
+      spec_state. iModIntro.
+
+      construct_wp_nonret.
+      edestruct H; first eassumption.
+      iSpecialize ("Hm" $! σ' m' μ Hstep0).
+      ewp_mask_elim. iMod "Hm" as "(Hewp & $)".
+      (* Use atomicity. *)
+      destruct m'; try discriminate H0;
+        ewp_unfold_all;
+        by iDestruct "Hewp" as ">>$". }
+    { admit. }
+  Admitted.
+
+  (** Derived rules *)
+
+  Lemma ewp_mono E m Ψ Q' Q : (∀ o, Q' o ⊢ Q o) → ewp_def E m Ψ Q' ⊢ ewp_def E m Ψ Q.
+  Proof.
+    iIntros (HΦ) "H"; ewp_mono with "H".
+    iIntros (v) "?". by iApply HΦ.
+  Qed.
+
+  Lemma ewp_mask_mono E1 E2 m Ψ Q :
+    E1 ⊆ E2 →
+    ewp_def E1 m Ψ Q ⊢ ewp_def E2 m Ψ Q.
+  Proof. iIntros (?) "H". ewp_mono with "H". Qed.
+
+  Global Instance ewp_mono' E m Ψ :
+    Proper (pointwise_relation _ (⊢) ==> (⊢)) (ewp_def E m Ψ).
+  Proof. by intros Φ Φ' ?; apply ewp_mono. Qed.
+
+  Global Instance ewp_flip_mono' E m Ψ :
+    Proper (pointwise_relation _ (CRelationClasses.flip (⊢)) ==> (CRelationClasses.flip (⊢))) (ewp_def E m Ψ).
+  Proof. by intros Φ Φ' ?; apply ewp_mono. Qed.
+
+  Lemma ewp_frame_l E m Ψ Φ R : R ∗ ewp_def E m Ψ Φ ⊢ ewp_def E m Ψ (λ o, R ∗ Φ o).
+  Proof. iIntros "[? H]". iApply (ewp_strong_mono with "H"); auto with iFrame. iApply iEff_le_refl. Qed.
+  Lemma ewp_frame_r E m Ψ Φ R : ewp_def E m Ψ Φ ∗ R ⊢ ewp_def E m Ψ (λ o, Φ o ∗ R).
+  Proof. iIntros "[H ?]". iApply (ewp_strong_mono with "H"); auto with iFrame. iApply iEff_le_refl. Qed.
+
+  Lemma ewp_wand E m Ψ Q' Q :
+    ewp_def E m Ψ Q' -∗ (∀ v, Q' v -∗ Q v) -∗ ewp_def E m Ψ Q.
+  Proof.
+    iIntros "Hwp H". ewp_mono with "Hwp".
+    iIntros (?) "?". by iApply "H".
+  Qed.
+  Lemma ewp_wand_l E m Ψ Q' Q :
+    (∀ v, Q' v -∗ Q v) ∗ ewp_def E m Ψ Q' ⊢ ewp_def E m Ψ Q.
+  Proof. iIntros "[H Hwp]". iApply (ewp_wand with "Hwp H"). Qed.
+  Lemma ewp_wand_r E m Ψ Q' Q :
+    ewp_def E m Ψ Q' ∗ (∀ v, Q' v -∗ Q v) ⊢ ewp_def E m Ψ Q.
+  Proof. iIntros "[Hwp H]". iApply (ewp_wand with "Hwp H"). Qed.
+  Lemma ewp_frame_wand E m Ψ Φ R :
+    R -∗ ewp_def E m Ψ (λ o, R -∗ Φ o) -∗ ewp_def E m Ψ Φ.
+  Proof.
+    iIntros "HR HWP". iApply (ewp_wand with "HWP").
+    iIntros (v) "HΦ". by iApply "HΦ".
+  Qed.
+
+End ewp.
 
 (* ------------------------------------------------------------------------ *)
 
@@ -85,185 +268,10 @@ Section ewp_basic_rules.
     by destruct o.
   Qed.
 
-  (* ------------------------------------------------------------------------ *)
-
-  Lemma ewp_step {σ π σ'} m m' μ :
-    thread_step (σ, m, dom π) (σ', m', μ) →
-    state_interp (σ, π) -∗
-    ewp_def E m Ψ Q ==∗
-    |={E}[∅]▷=>
-        ewp_def E m' Ψ Q ∗
-          (match μ with
-           | None => state_interp (σ', π)
-           | Some (ι', m') => ∃ φ' γ, state_interp (σ', <[ι':= γ]>π) ∗
-                                        saved_prop.saved_pred_own γ DfracDiscarded φ' ∗
-                                        ewp_def E m' ⊥ (λ o, □ φ' o)
-          end).
-  Proof.
-    intros Hstep.
-    iIntros "Hsi Hwp".
-    ewp_unfold m.
-    ewp_case m.
-    spec_state. iModIntro. iMod "Hwp" as "[%Hprog Hwp]".
-    spec_step.
-    by ewp_mask_elim.
-  Qed.
-
-  (* ------------------------------------------------------------------------ *)
-
-  (** Monotonicity. *)
-  Lemma ewp_mono m Q' :
-    ewp_def E m Ψ Q' -∗
-    (∀ o, Q' o -∗ Q o) -∗
-    ewp_def E m Ψ Q.
-  Proof.
-    iIntros "Hwp Hmono".
-    iLöb as "IH" forall (m).
-    ewp_unfold m.
-    ewp_case m.
-    (* Case: [m] is a [WPOutcome] *)
-    { iMod "Hwp"; iModIntro.
-      iApply ("Hmono" with "Hwp"). }
-
-    (* Case: [m] is a [WPCrash]. *)
-    { done. }
-
-    { (* Case: [m] is a [WPPerform]. We use [prot_mono]. *)
-      iMod "Hwp"; iModIntro.
-      iApply (monotonic_prot with "[-Hwp] Hwp").
-      iIntros (w) "Hwp !>".
-      by iApply ("IH" with "Hwp Hmono"). }
-
-    { (* Case: [m] is a [WPStep]. *)
-      intro_state. spec_state. iModIntro.
-      discharge_pure assumption.
-      clear Hstep.
-      iIntros (σ' m' μ) "%Hstep".
-      spec_step.
-      ewp_mask_elim. iMod "Hwp" as "(Hwp & Hforked)". iFrame.
-      iApply ("IH" with "Hwp Hmono"). }
-
-    { (* Case: [m] is a [WPJoin]. *)
-      intro_state. spec_state.
-      iMod "Hwp". iModIntro.
-      destruct (π !! t) eqn:Hlookup; last done.
-      iDestruct "Hwp" as "(%φ'0 & $ & Hwp)".
-      iIntros "!> %o Ho". iSpecialize ("Hwp" with "Ho").
-      ewp_mask_elim. iMod "Hwp" as "(Hwp & Hforked)". iFrame.
-      iApply ("IH" with "Hwp Hmono"). }
-  Qed.
-
-  Lemma ewp_prot_mono m Ψ' :
-    (Ψ' ⊑ Ψ)%ieff -∗
-    ewp_def E m Ψ' Q -∗
-    ewp_def E m Ψ Q.
-  Proof.
-    iIntros "#Hmono Hwp".
-    iLöb as "IH" forall (m).
-    ewp_unfold m.
-    ewp_case m; try done.
-
-    { (* Case: [m] is a [WPPerform]. We use [prot_mono]. *)
-      iMod "Hwp"; iModIntro.
-      iDestruct "Hwp" as (φ) "(Hwp & HΨ)"; iExists φ.
-      iSplitL "Hwp"; first iApply ("Hmono" with "Hwp"); cbn.
-      iIntros (?) "Hφ". iSpecialize ("HΨ" with "Hφ").
-      iNext; iApply ("IH" with "HΨ"). }
-
-    { (* Case: [m] is a [WPStep]. *)
-      intro_state. spec_state. iModIntro.
-      construct_wp_nonret. spec_step.
-      ewp_mask_elim.
-      iMod "Hwp" as "(Hwp & $)".
-      by iApply ("IH" with "Hwp"). }
-
-    { (* Case: [m] is a [WPJoin]. *)
-      intro_state. spec_state. iMod "Hwp"; iModIntro.
-      destruct (π !! t); last done.
-      iDestruct "Hwp" as "(%φ'0 & $ & Hwp)".
-      iIntros "!> %o Ho". iSpecialize ("Hwp" with "Ho").
-      ewp_mask_elim.
-      iMod "Hwp" as "(Hwp & $)".
-      by iApply ("IH" with "Hwp"). }
-  Qed.
-
-  Lemma ewp_pers_smono m E' Q' :
-    E' ⊆ E →
-    ewp_def E' m Ψ Q' -∗
-    □ (∀ v, Q' v ={E}=∗ Q v) -∗
-    ewp_def E m Ψ Q.
-  Proof.
-    iIntros (HE) "He HΦ".
-    iRevert "HΦ".
-    iLöb as "IH" forall (A X m Ψ Q Q').
-    iIntros "#HΦ".
-    ewp_unfold m.
-    ewp_case m.
-    { (* Cases: [WPOutcome] *)
-      iApply ("HΦ" with "[> -]"); by iApply (fupd_mask_mono E' E). }
-    (* Case: [WPCrash] *)
-    { by iApply (fupd_mask_mono E' E). }
-    (* Case: [WPPerform] *)
-    { iApply (fupd_mask_mono E' E); first done.
-      iMod "He"; iModIntro.
-      iApply (monotonic_prot with "[-He] He").
-      iIntros (o) "Hwp !>".
-      iApply ("IH" with "Hwp HΦ"). }
-    { (* Case: [WPStep] *)
-      intro_state.
-      iMod (fupd_mask_subseteq E') as "Hclose"; first done.
-      spec_state. iModIntro. construct_wp_nonret.
-      spec_step. ewp_mask_elim.
-      iDestruct "He" as ">(H & Hforked)".
-      iMod "Hclose"; iModIntro.
-      iSplitL "H"; first by iApply ("IH" with "H HΦ").
-      destruct μ as [ [ι' mforked] | ]; last iFrame.
-      iDestruct "Hforked" as "(%φ' & %γ & Hsi & Hsaved & Hwp)".
-      iFrame. iApply ("IH" with "Hwp").
-      auto. }
-    { (* Case: [WPJoin] *)
-      intro_state.
-      iMod (fupd_mask_subseteq E') as "Hclose"; first done.
-      spec_state. iMod "He"; iModIntro.
-      destruct (π !! t).
-      - iDestruct "He" as "(%φ' & $ & He)".
-        iIntros "!> %o Ho". iSpecialize ("He" with "Ho").
-        ewp_mask_elim.
-        iDestruct "He" as ">(H & Hforked)".
-        iMod "Hclose"; iModIntro. iFrame.
-        iApply ("IH" with "H HΦ").
-      - iMod "He". iMod "Hclose". iModIntro. done. }
-  Qed.
-
-  Lemma ewp_pers_mono m Q' :
-    ewp_def E m Ψ Q' -∗
-    □ (∀ o, Q' o ={E}=∗ Q o) -∗
-    ewp_def E m Ψ Q.
-  Proof.
-    iIntros "He #Hmono".
-    iApply (ewp_pers_smono with "He"). set_solver.
-    by iIntros "!>".
-  Qed.
-
-  (* Eliminate update modality in postcondition *)
-  Lemma ewp_fupd_post m :
-    ewp_def E m Ψ (λ o, |={E}=> Q o) -∗
-    ewp_def E m Ψ Q.
-  Proof.
-    iIntros "He".
-    iApply (ewp_pers_mono with "He"); auto.
-  Qed.
-
-  Lemma ewp_fupd m :
-    (|={E}=> ewp_def E m Ψ Q) -∗
-    ewp_def E m Ψ Q.
-  Proof.
-    iIntros "He".
-    ewp_unfold_all.
-    ewp_case m; try iMod "He"; done.
-  Qed.
-
 End ewp_basic_rules.
+
+
+
 
 (* ------------------------------------------------------------------------ *)
 (* Invert cases where there are premises of the form
@@ -575,10 +583,10 @@ Section ewp_rules.
     (* The result is immediate. *)
     { rewrite try2_inject2.
       iPoseProof (ewp_outcome2_inv with "Hwp") as "Hret"; cbn.
-      iApply (ewp_fupd with "Hret"). }
+      iApply (fupd_ewp with "Hret"). }
     (* Case : [m1] is [crash]; trivial  *)
     { iClear "IH".
-      iApply ewp_fupd.
+      iApply fupd_ewp.
       ewp_unfold (@Crash A X); by iMod "Hwp". }
     (* Case : [m1] is [Perform _ _]. *)
     { cbn.
@@ -716,7 +724,7 @@ Section ewp_rules.
       - (* [ParPerformLeft] *)
         ewp_mask_intro "Hmod"; ewp_mask_elim; iFrame.
         iPoseProof (ewp_perform_inv with "[$]") as "H1".
-        iApply ewp_fupd. iMod "H1"; iModIntro.
+        iApply fupd_ewp. iMod "H1"; iModIntro.
         iApply ewp_stop_perform.
         iApply (monotonic_prot with "[H2 Hjoin] H1").
         iIntros (?) "Hk".
@@ -750,7 +758,7 @@ Section ewp_rules.
       - (* [StepParPerformRight] *)
         ewp_mask_intro "Hmod"; ewp_mask_elim; iFrame.
         iPoseProof (ewp_perform_inv with "[$]") as "H2".
-        iApply ewp_fupd. iMod "H2"; iModIntro.
+        iApply fupd_ewp. iMod "H2"; iModIntro.
         iApply ewp_stop_perform.
         iApply (monotonic_prot with "[H1 Hjoin] H2").
         iIntros (?) "H2".
@@ -841,8 +849,7 @@ Section ewp_val_rules.
     ⊢ imp m ⟨⟨ λ e, ⌜ζ e⌝ ⟩⟩ {{ λ x, ⌜φ x⌝ }} .
   Proof.
     iIntros (Hpure).
-    iApply ewp_mono.
-    iApply pure_ewp. apply Hpure.
+    iApply ewp_mono; last (iApply pure_ewp; apply Hpure).
     iIntros ([v|e]).
     - iIntros "(%a & %Henc & %Ha)".
       iPureIntro.
